autoclrs/ch09-order-statistics/CLRS.Ch09.PartialSelectionSort.Impl.fsti
@@ -13,6 +13,7 @@ module A = Pulse.Lib.Array
 module SZ = FStar.SizeT
 module Seq = FStar.Seq
 module GR = Pulse.Lib.GhostReference
+module PSSSpec = CLRS.Ch09.PartialSelectionSort.Spec
 
 [@@"opaque_to_smt"]
 let permutation (s1 s2: Seq.seq int) : prop = (Seq.Properties.permutation int s1 s2)
@@ -87,5 +88,6 @@ fn select
       prefix_leq_suffix s_final (SZ.v k) /\
       SZ.v k > 0 /\
       result == Seq.index s_final (SZ.v k `Prims.op_Subtraction` 1) /\
+      result == PSSSpec.select_spec s0 (SZ.v k `Prims.op_Subtraction` 1) /\
       complexity_bounded_select cf (reveal c0) (SZ.v n) (SZ.v k)
     )
